src/Turing.v
@@ -35,20 +35,17 @@ Require Import Coq.Logic.Classical_Prop.
 
   Definition lang := input -> Prop.
 
-  (** The result of running a Turing machine. *)
-  Inductive result :=
-    | Halt: bool -> result
-    | Loop: result.
-
   (** We can run a machine and obtain its run result. *)
-  Parameter Exec: machine -> input -> result -> Prop.
-  Parameter exec_fun: forall m i r1 r2,
-    Exec m i r1 ->
-    Exec m i r2 ->
-    r1 = r2.
+  Parameter Exec: machine -> input -> bool -> Prop.
+
+  Parameter exec_fun: forall m i b1 b2,
+    Exec m i b1 ->
+    Exec m i b2 ->
+    b1 = b2.
+
   Parameter exec_exists:
     forall m i,
-    exists r, Exec m i r.
+    (exists b, Exec m i b) \/ (forall b, ~ Exec m i b).
 
   Inductive Prog :=
   | Read: (input -> Prog) -> Prog
@@ -68,7 +65,7 @@ Require Import Coq.Logic.Classical_Prop.
       This Turing Machine just accepts/loops/rejects without
       any further operation.
       *)
-  | Ret: result -> Prog
+  | Ret: bool -> Prog
   .
 
   (**
@@ -76,46 +73,459 @@ Require Import Coq.Logic.Classical_Prop.
     We can run a program `p` and obtain a resul `r` with
     `Run p r`.
     *)
-  Inductive Run: Prog -> input -> result -> Prop :=
+  Inductive Run: Prog -> input -> bool -> Prop :=
   | run_read:
-    forall p i r,
-    Run (p i) i r ->
-    Run (Read p) i r
+    forall p i b,
+    Run (p i) i b->
+    Run (Read p) i b
   | run_call:
-    forall p i j r,
-    Run p i r ->
-    Run (Call p i) j r 
+    forall p i j b,
+    Run p i b ->
+    Run (Call p i) j b 
   | run_ret:
     (** We can directly return a result *)
-    forall r i,
-    Run (Ret r) i r
+    forall b i,
+    Run (Ret b) i b
   | run_tur:
-    (** Calling a machine is the same as using function `run`. *)
-    forall m i r,
-    Exec m i r ->
-    Run (Tur m) i r
-  | run_seq_cont:
+    (** Run a turing machine `m`. *)
+    forall m i b,
+    Exec m i b ->
+    Run (Tur m) i b
+  | run_seq:
     (** If `p` terminates and returns `b`, then we can
        proceed with the execution of `q b`. *) 
-    forall p q b r i,
-    Run p i (Halt b) ->
-    Run (q b) i r ->
-    Run (Seq p q) i r
-  | run_seq_loop:
-    (** If `p` loops, then `p; q` also loops. *)
+    forall p q b1 b2 i,
+    Run p i b1 ->
+    Run (q b1) i b2 ->
+    Run (Seq p q) i b2.
+
+  Inductive Halt : Prog -> input -> Prop :=
+  | halt_read:
+    forall p i,
+    Halt (p i) i ->
+    Halt (Read p) i
+  | halt_call:
+    forall p i j,
+    Halt p i ->
+    Halt (Call p i) j 
+  | halt_ret:
+    (** We can directly return a result *)
+    forall i b,
+    Halt (Ret b) i
+  | halt_tur:
+    (** Run a turing machine `m`. *)
+    forall m i b,
+    Exec m i b ->
+    Halt (Tur m) i
+  | halt_seq:
+    (** If `p` terminates and returns `b`, then we can
+       proceed with the execution of `q b`. *) 
+    forall p q b i,
+    Run p i b ->
+    Halt (q b) i ->
+    Halt (Seq p q) i.
+
+  Inductive Loop: Prog -> input -> Prop :=
+  | loop_read:
+    forall p i,
+    Loop (p i) i ->
+    Loop (Read p) i
+  | loop_call:
+    forall p i j,
+    Loop p i ->
+    Loop (Call p i) j
+  | loop_tur:
+    (** Run a turing machine `m`. *)
+    forall m i,
+    (forall b, ~ Exec m i b) ->
+    Loop (Tur m) i
+  | loop_seq_l:
+    (** If `p` terminates and returns `b`, then we can
+       proceed with the execution of `q b`. *) 
     forall p q i,
-    Run p i Loop ->
-    Run (Seq p q) i Loop.
+    Loop p i ->
+    Loop (Seq p q) i
+  | loop_seq_r:
+    (** If `p` terminates and returns `b`, then we can
+       proceed with the execution of `q b`. *) 
+    forall p q b i,
+    Run p i b ->
+    Loop (q b) i ->
+    Loop (Seq p q) i.
+
+  Inductive Negative p i : Prop :=
+  | negative_run_false:
+    Run p i false ->
+    Negative p i
+  | negative_loop:
+    Loop p i ->
+    Negative p i.
 
   (** We define a notation for sequencing. *)
   Notation "'mlet' x <- e 'in' c" := (Seq e (fun x => c)) (at level 60, right associativity).
 
-  (** Notation for ACCEPT means returning Accept *)
-  Notation ACCEPT := (Ret (Halt true)).
-  (** Notation for LOOP means returning Reject *)
-  Notation REJECT := (Ret (Halt false)).
-  (** Notation for LOOP means returning Loop *)
-  Notation LOOP := (Ret Loop).
+  Lemma run_read_rw:
+    forall f i b,
+    Run (Read f) i b <-> Run (f i) i b.
+  Proof.
+    split; intros.
+    - inversion H; subst; auto.
+    - constructor; assumption.
+  Qed.
+
+  Lemma run_call_rw:
+    forall p i j b,
+    Run (Call p j) i b <-> Run p j b.
+  Proof.
+    split; intros.
+    - inversion H; subst; auto.
+    - constructor; auto.
+  Qed.
+
+  Lemma halt_read_rw:
+    forall f i,
+    Halt (Read f) i <-> Halt (f i) i.
+  Proof.
+    split; intros.
+    - inversion H; subst; auto.
+    - constructor; assumption.
+  Qed.
+
+  Lemma halt_call_rw:
+    forall p i j,
+    Halt (Call p j) i <-> Halt p j.
+  Proof.
+    split; intros.
+    - inversion H; subst; auto.
+    - constructor; auto.
+  Qed.
+
+  (*----------------------------------------------------------------------------*)
+
+  Section RunLoopHalt.
+
+    Lemma run_fun:
+      forall p i b1,
+      Run p i b1 ->
+      forall b2,
+      Run p i b2 ->
+      b1 = b2.
+    Proof.
+      intros p i r1 H; induction H; intros r' He;
+        inversion He; subst; clear He; auto;
+        (* In each case we have a bunch of Run's that are solved
+           by induction; we need to make sure we clear any dec's,
+           so that we can advance to the next IH *) 
+        repeat match goal with
+        | [ H1: Run ?q i ?b1, H2: Run ?q i ?b2 |- _] =>
+          (
+            assert (b1 = b2) by eauto ||
+            assert (b2 = b1) by eauto
+          ); subst; clear H2; auto
+        end;
+        auto.
+      eauto using exec_fun.
+    Qed.
+
+    Lemma halt_to_run:
+      forall p i,
+      Halt p i ->
+      exists b, Run p i b.
+    Proof.
+      intros.
+      induction H; try destruct IHHalt as (b, Hr).
+      - exists b.
+        constructor.
+        assumption.
+      - exists b.
+        constructor.
+        assumption.
+      - exists b.
+        constructor.
+      - exists b.
+        constructor.
+        assumption.
+      - destruct IHHalt as (b1, Hr).
+        exists b1.
+        econstructor; eauto.
+    Qed.
+
+    Lemma run_to_halt:
+      forall p i b,
+      Run p i b ->
+      Halt p i.
+    Proof.
+      intros.
+      induction H.
+      - constructor.
+        assumption.
+      - constructor.
+        assumption.
+      - constructor.
+      - eapply halt_tur; eauto.
+      - eapply halt_seq; eauto.
+    Qed.
+
+    Lemma halt_rw:
+      forall p i,
+      Halt p i <-> exists b, Run p i b.
+    Proof.
+      split; intros.
+      - auto using halt_to_run.
+      - destruct H.
+        eauto using run_to_halt.
+    Qed.
+
+    Lemma halt_or_loop:
+      forall p i,
+      Halt p i \/ Loop p i.
+    Proof.
+      induction p; intros.
+      - assert (H := H i i).
+        destruct H as [H| H].
+        + left.
+          constructor.
+          assumption.
+        + right.
+          constructor.
+          assumption.
+      - assert (IHp := IHp i).
+        destruct IHp as [H|H]. {
+          left.
+          constructor.
+          assumption.
+        }
+        right.
+        constructor.
+        assumption.
+      - assert (IHp := IHp i).
+        destruct IHp as [IH|IH].
+        + apply halt_to_run in IH.
+          destruct IH as (b, IH).
+          assert (H := H b i).
+          destruct H as [H|H]. {
+            left.
+            econstructor; eauto.
+          }
+          right.
+          eapply loop_seq_r; eauto.
+        + right.
+          eauto using loop_seq_l.
+      - destruct (exec_exists m i) as [(b, He)|Hl]. {
+          left.
+          econstructor.
+          eauto.
+        }
+        right.
+        constructor.
+        auto.
+      - left.
+        constructor.
+    Qed.
+
+    Lemma loop_to_not_halt:
+      forall p i,
+      Loop p i ->
+      ~ Halt p i.
+    Proof.
+      intros; induction H; intros N; inversion_clear N;
+        try (contradict IHLoop; auto; fail).
+      - apply H in H0.
+        assumption.
+      - contradict IHLoop.
+        eapply run_to_halt; eauto.
+      - assert (b0 = b) by eauto using run_fun.
+        subst.
+        contradiction.
+    Qed.
+
+    Lemma halt_to_not_loop:
+      forall p i,
+      Halt p i ->
+      ~ Loop p i.
+    Proof.
+      intros.
+      induction H; intros N.
+      - inversion_clear N.
+        contradict H.
+        auto.
+      - inversion_clear N.
+        contradiction.
+      - inversion_clear N.
+      - inversion_clear N.
+        contradict H.
+        auto.
+      - inversion_clear N. {
+          apply loop_to_not_halt in H1.
+          contradict H1.
+          eapply run_to_halt; eauto.
+        }
+        assert (b0 = b) by eauto using run_fun.
+        subst.
+        contradiction.
+    Qed.
+
+    Lemma not_halt_to_loop:
+      forall p i,
+      ~ Halt p i ->
+      Loop p i.
+    Proof.
+      intros.
+      destruct (halt_or_loop p i). {
+        contradiction.
+      }
+      assumption.
+    Qed.
+
+    Lemma loop_rw:
+      forall p i,
+      Loop p i <-> ~ Halt p i.
+    Proof.
+      split; intros. {
+        auto using loop_to_not_halt.
+      }
+      auto using not_halt_to_loop.
+    Qed.
+
+    Lemma loop_read_rw:
+      forall p i,
+      Loop (Read p) i <-> Loop (p i) i.
+    Proof.
+      split; intros. {
+        inversion_clear H.
+        assumption.
+      }
+      auto using loop_read.
+    Qed.
+
+    Lemma loop_call_rw:
+      forall p i j,
+      Loop (Call p j) i <-> Loop p j.
+    Proof.
+      split; intros. {
+        inversion_clear H.
+        assumption.
+      }
+      auto using loop_call.
+    Qed.
+
+    Lemma run_exists:
+      forall p i,
+      (exists b, Run p i b) \/ Loop p i.
+    Proof.
+      intros.
+      destruct (halt_or_loop p i); auto.
+      rewrite halt_rw in *.
+      auto.
+    Qed.
+
+    Lemma loop_alt_rw:
+      forall p i,
+      Loop p i <-> (forall b, ~ Run p i b).
+    Proof.
+      split; intros. {
+        rewrite loop_rw in H.
+        intros N.
+        contradict H.
+        eauto using run_to_halt.
+      }
+      rewrite loop_rw.
+      intros N.
+      rewrite halt_rw in N.
+      destruct N as (b, N).
+      apply H in N.
+      contradiction.
+    Qed.
+
+    Lemma negative_alt_rw:
+      forall p i,
+      Negative p i <-> (Run p i false \/ Loop p i).
+    Proof.
+      split; intros. { inversion_clear H; auto. }
+      destruct H. { auto using negative_run_false. }
+      auto using negative_loop.
+    Qed.
+
+    Lemma negative_rw:
+      forall p i,
+      Negative p i <-> ~ Run p i true.
+    Proof.
+      split; intros. {
+        intros N.
+        inversion_clear H. {
+          assert (X: true = false) by eauto using run_fun.
+          inversion X.
+        }
+        rewrite loop_rw in *.
+        contradict H0.
+        eapply run_to_halt; eauto.
+      }
+      destruct (halt_or_loop p i). {
+        rewrite halt_rw in *.
+        destruct H0 as ([], Ha); try contradiction.
+        auto using negative_run_false.
+      }
+      auto using negative_loop.
+    Qed.
+
+    Lemma negative_read_rw:
+      forall p i,
+      Negative (Read p) i <-> Negative (p i) i.
+    Proof.
+      split; intros. {
+        inversion_clear H. {
+          rewrite run_read_rw in *.
+          auto using negative_run_false.
+        }
+        rewrite loop_read_rw in *.
+        auto using negative_loop.
+      }
+      rewrite negative_alt_rw in H.
+      destruct H. {
+        apply negative_run_false.
+        rewrite run_read_rw.
+        assumption.
+      }
+      apply negative_loop.
+      rewrite loop_read_rw.
+      assumption.
+    Qed.
+
+    Lemma negative_call_rw:
+      forall p i j,
+      Negative (Call p j) i <-> Negative p j.
+    Proof.
+      split; intros. {
+        inversion_clear H. {
+          rewrite run_call_rw in *.
+          auto using negative_run_false.
+        }
+        rewrite loop_call_rw in *.
+        auto using negative_loop.
+      }
+      rewrite negative_alt_rw in H.
+      destruct H. {
+        apply negative_run_false.
+        rewrite run_call_rw.
+        assumption.
+      }
+      apply negative_loop.
+      rewrite loop_call_rw.
+      assumption.
+    Qed.
+
+    Lemma run_true_or_negative:
+      forall p i,
+      Run p i true \/ Negative p i.
+    Proof.
+      intros.
+      destruct (run_exists p i) as [([], H)|H];
+        auto;
+        right;
+        auto using negative_run_false, negative_loop.
+    Qed.
+
+  End RunLoopHalt.
 
   (** We also define a function to serialize a machine into a string (of type
       input). In the book, this corresponds to notation <M>. *)
@@ -224,12 +634,12 @@ Require Import Coq.Logic.Classical_Prop.
        *)
 
   Definition Recognizes (p:Prog) (L:lang) :=
-    forall i, Run p i (Halt true) <-> L i.
+    forall i, Run p i true <-> L i.
 
   Lemma recognizes_def:
     forall p (L:lang),
-    (forall i, Run p i (Halt true) -> L i) ->
-    (forall i, L i -> Run p i (Halt true)) ->
+    (forall i, Run p i true -> L i) ->
+    (forall i, L i -> Run p i true) ->
     Recognizes p L.
   Proof.
     intros.
@@ -332,104 +742,18 @@ Require Import Coq.Logic.Classical_Prop.
     assumption.
   Qed.
 
-
-  Lemma run_read_rw:
-    forall f i r,
-    Run (Read f) i r <-> Run (f i) i r.
-  Proof.
-    split; intros.
-    - inversion H; subst; auto.
-    - constructor; assumption.
-  Qed.
-
-  Lemma run_call_rw:
-    forall p i j r,
-    Run (Call p j) i r <-> Run p j r.
-  Proof.
-    split; intros.
-    - inversion H; subst; auto.
-    - constructor; auto.
-  Qed.
-
-  (*----------------------------------------------------------------------------*)
-
   Section RecognizesRun.
-
-    Ltac clear_result :=
-      match goal with
-        | [ H: Halt _ = Loop |- _ ] =>
-          inversion H
-        | [ H: Loop = Halt _ |- _ ] => inversion H
-        | [ H: Loop = Loop |- _ ] => clear H
-        | [ H1: Halt ?b1 = Halt ?b2 |- _] =>
-          inversion H1; subst; clear H1
-        end.
-
-    Lemma run_fun:
-      forall p i r1,
-      Run p i r1 ->
-      forall r2,
-      Run p i r2 ->
-      r1 = r2.
-    Proof.
-      intros p i r1 H; induction H; intros r' He;
-        inversion He; subst; clear He; auto;
-        (* In each case we have a bunch of Run's that are solved
-           by induction; we need to make sure we clear any dec's,
-           so that we can advance to the next IH *) 
-        repeat match goal with
-        | [ H1: Run ?q i ?r1, H2: Run ?q i ?r2 |- _] =>
-          (
-            assert (r1 = r2) by eauto ||
-            assert (r2 = r1) by eauto
-          ); subst; clear H2; try clear_result; auto
-        end;
-        try clear_result;
-        auto.
-      eauto using exec_fun.
-    Qed.
-
-    Lemma run_exists:
-      forall p i,
-      exists r, Run p i r.
-    Proof.
-      induction p; intros.
-      - assert (H := H i i).
-        destruct H as (r, Hr).
-        exists r.
-        constructor; auto.
-      - assert (IHp := IHp i).
-        destruct IHp as (r, IHp).
-        exists r.
-        constructor.
-        assumption.
-      - assert (IHp := IHp i).
-        destruct IHp as ([], IHp).
-        + assert (H := H b i).
-          destruct H as (r, H).
-          exists r.
-          eapply run_seq_cont; eauto.
-        + exists Loop.
-          constructor.
-          assumption.
-      - destruct (exec_exists m i) as (r, He).
-        exists r.
-        constructor.
-        assumption.
-      - exists r.
-        constructor.
-    Qed.
 
     Lemma recognizes_run_reject:
       forall p L i,
       Recognizes p L ->
-      Run p i (Halt false) ->
+      Run p i false ->
       ~ L i.
     Proof.
       intros.
       intros N.
       apply H in N.
-      assert (Hx: Halt true = Halt false) by eauto using run_fun.
+      assert (Hx: true = false) by eauto using run_fun.
       inversion Hx.
     Qed.
 
@@ -437,7 +761,7 @@ Require Import Coq.Logic.Classical_Prop.
       forall p L,
       Recognizes p L ->
       forall i,
-      Run p i (Halt true) ->
+      Run p i true ->
       L i.
     Proof.
       intros.
@@ -447,10 +771,11 @@ Require Import Coq.Logic.Classical_Prop.
 
 
     Lemma recognizes_not_accept:
-      forall p L i,
+      forall p L,
       Recognizes p L ->
+      forall i,
       ~ L i ->
-      ~ Run p i (Halt true).
+      ~ Run p i true.
     Proof.
       intros.
       intros N.
@@ -458,11 +783,23 @@ Require Import Coq.Logic.Classical_Prop.
       contradiction.
     Qed.
 
+    Lemma recognizes_negative:
+      forall p L,
+      Recognizes p L ->
+      forall i,
+      ~ L i ->
+      Negative p i.
+    Proof.
+      intros.
+      rewrite negative_rw.
+      eauto using recognizes_not_accept.
+    Qed.
+
     Lemma recognizes_accept:
       forall p L i,
       Recognizes p L ->
       L i ->
-      Run p i (Halt true).
+      Run p i true.
     Proof.
       intros.
       apply H in H0.
@@ -473,21 +810,34 @@ Require Import Coq.Logic.Classical_Prop.
       forall p L,
       Recognizes p L ->
       forall i,
-      Run p i Loop ->
+      Loop p i ->
       ~ L i.
     Proof.
       intros.
       intros N.
       apply H in N.
-      assert (Hx: Loop = Halt true) by eauto using run_fun.
-      inversion Hx.
+      apply halt_to_not_loop in H0; auto.
+      eauto using run_to_halt.
+    Qed.
+
+    Lemma recognizes_inv_negative:
+      forall p L,
+      Recognizes p L ->
+      forall i,
+      Negative p i ->
+      ~ L i.
+    Proof.
+      intros.
+      inversion_clear H0.
+      - eauto using recognizes_run_reject.
+      - eauto using recognizes_run_loop.
     Qed.
 
     Lemma recognizes_accept_rw:
       forall p L,
       Recognizes p L ->
       forall i,
-      Run p i (Halt true) <-> L i.
+      Run p i true <-> L i.
     Proof.
       split; intros.
       - eapply recognizes_run_accept; eauto.
@@ -507,6 +857,7 @@ Require Import Coq.Logic.Classical_Prop.
         symmetry.
         auto.
     Qed.
+
   End RecognizesRun.
 
   (*----------------------------------------------------------------------------*)
@@ -535,7 +886,7 @@ Require Import Coq.Logic.Classical_Prop.
     Lemma co_recognizes_run_accept:
       forall m L i,
       Recognizes m (compl L) ->
-      Run m i (Halt true) ->
+      Run m i true ->
       ~ L i.
     Proof.
       intros.
@@ -546,7 +897,7 @@ Require Import Coq.Logic.Classical_Prop.
       forall m L i,
       Recognizes m (compl L) ->
       L i ->
-      ~ Run m i (Halt true).
+      ~ Run m i true.
     Proof.
       intros.
       intros N.
@@ -558,7 +909,7 @@ Require Import Coq.Logic.Classical_Prop.
       forall m L i,
       Recognizes m (compl L) ->
       ~ L i ->
-      Run m i (Halt true).
+      Run m i true.
     Proof.
       intros.
       unfold compl in *.
@@ -573,11 +924,12 @@ Require Import Coq.Logic.Classical_Prop.
   Section Decidable.
     (** We define a decider as any Turing Machine that returns either Accept or
         Reject, but not Loop. *)
-    Definition Decider (p:Prog) := forall i, exists b, Run p i (Halt b).
+
+    Definition Decider (p:Prog) := forall i, Halt p i.
 
     Lemma decider_def:
       forall p,
-      (forall i, exists b, Run p i (Halt b)) ->
+      (forall i, Halt p i) ->
       Decider p.
     Proof.
       intros.
@@ -642,7 +994,7 @@ Require Import Coq.Logic.Classical_Prop.
     Lemma decides_run_reject:
       forall m L i,
       Decides m L ->
-      Run m i (Halt false) ->
+      Run m i false ->
       ~ L i.
     Proof.
       intros.
@@ -653,7 +1005,7 @@ Require Import Coq.Logic.Classical_Prop.
     Lemma decides_run_accept:
       forall m L i,
       Decides m L ->
-      Run m i (Halt true) ->
+      Run m i true ->
       L i.
     Proof.
       intros.
@@ -665,56 +1017,80 @@ Require Import Coq.Logic.Classical_Prop.
       forall m L i,
       Decides m L ->
       L i ->
-      Run m i (Halt true).
+      Run m i true.
     Proof.
       intros.
       apply decides_to_recognizes in H.
       apply recognizes_accept with (L:=L); auto.
     Qed.
 
-    Lemma decides_inv_run_result:
-      forall p L,
-      Decides p L ->
-      forall i r,
-      Run p i r ->
-      exists b, r = Halt b.
-    Proof.
-      intros.
-      destruct H as (Ha, Hb).
-      destruct (Hb i);
-      eauto using run_fun.
-    Qed.
-
-    Lemma decider_to_run:
+    Lemma decider_to_halt:
       forall p,
       Decider p ->
       forall i,
-      exists b, Run p i (Halt b).
+      Halt p i.
     Proof.
       intros.
       unfold Decider in *.
       auto.
     Qed.
 
+    Lemma decider_to_run:
+      forall p i,
+      Decider p ->
+      Run p i true \/ Run p i false.
+    Proof.
+      intros.
+      apply decider_to_halt with (i:=i) in H.
+      rewrite halt_rw in *.
+      destruct H as ([], H); auto.
+    Qed.
+
     Lemma decides_to_run:
-      forall p L,
+      forall p L i,
       Decides p L ->
-      forall i,
-      exists b, Run p i (Halt b).
+      exists b, Run p i b.
     Proof.
       intros.
       destruct H.
-      eauto.
+      specialize (H0 i).
+      rewrite halt_rw in *.
+      assumption.
+    Qed.
+
+    Lemma decides_to_halt:
+      forall p L,
+      Decides p L ->
+      forall i,
+      Halt p i.
+    Proof.
+      intros.
+      destruct H.
+      unfold Decider in *.
+      auto.
+    Qed.
+
+    Lemma decider_to_not_loop:
+      forall p,
+      Decider p ->
+      forall i,
+      ~ Loop p i.
+    Proof.
+      intros.
+      specialize (H i).
+      auto using halt_to_not_loop.
     Qed.
 
     Lemma decider_not_reject:
       forall p i,
       Decider p ->
-      ~ Run p i (Halt false) ->
-      Run p i (Halt true).
+      ~ Run p i false ->
+      Run p i true.
     Proof.
       intros.
-      edestruct decider_to_run with (i:=i) as (b, Hr); eauto.
+      assert (H := H i).
+      rewrite halt_rw in *.
+      destruct H as (b, H).
       destruct b;
       intuition.
     Qed.
@@ -722,12 +1098,15 @@ Require Import Coq.Logic.Classical_Prop.
     Lemma decider_not_accept:
       forall m i,
       Decider m ->
-      ~ Run m i (Halt true) ->
-      Run m i (Halt false).
+      ~ Run m i true ->
+      Run m i false.
     Proof.
       intros.
-      edestruct decider_to_run with (i:=i) as (b, Hr); eauto.
-      destruct b; intuition.
+      assert (H := H i).
+      rewrite halt_rw in *.
+      destruct H as (b, H).
+      destruct b;
+      intuition.
     Qed.
 
     Lemma decides_to_decider:
@@ -744,150 +1123,20 @@ Require Import Coq.Logic.Classical_Prop.
       forall m L i,
       Decides m L ->
       ~ L i ->
-      Run m i (Halt false).
+      Run m i false.
     Proof.
       intros.
       destruct H.
-      apply decider_to_run with (i:=i) in H1.
-      destruct H1 as ([], Hr).
-      - apply recognizes_run_accept with (L:=L) in Hr; auto.
-        contradiction.
-      - assumption.
+      assert (Ha: Halt m i) by auto using decider_to_halt.
+      rewrite halt_rw in *.
+      destruct Ha as (b, Ha).
+      destruct b; auto.
+      contradict H0.
+      eapply recognizes_run_accept; eauto.
     Qed.
-
-    Lemma decider_no_loop:
-      forall m i,
-      Decider m ->
-      ~ Run m i Loop.
-    Proof.
-      intros.
-      unfold Decider in *.
-      intros N.
-      destruct (H i) as ([], Ha).
-      - assert (M: Loop = Halt true) by eauto using run_fun; inversion M.
-      - assert (M: Loop = Halt false) by eauto using run_fun; inversion M.
-    Qed.
-
-    Lemma decides_no_loop:
-      forall m L,
-      Decides m L ->
-      forall i,
-      ~ Run m i Loop.
-    Proof.
-      intros.
-      destruct H.
-      eapply decider_no_loop; eauto.
-    Qed.
-
 
   End Decidable.
 
-  (**
-    A Theory to reason about recognizability/decidability directly on
-    programs.
-    *)
-  Section HALTS.
-
-    (* A program halts *)
-    Inductive Halts: Prog -> input -> Prop :=
-    | halts_read:
-      forall p i,
-      Halts (p i) i ->
-      Halts (Read p) i
-    | halts_call:
-      forall p i j,
-      Halts p j ->
-      Halts (Call p j) i
-    | halts_ret:
-      forall i b,
-      Halts (Ret (Halt b)) i
-    | halts_tur:
-      forall m i b,
-      Exec m i (Halt b) ->
-      Halts (Tur m) i
-    | halts_seq:
-      forall p i b q,
-      Run p i (Halt b) ->
-      Halts (q b) i ->
-      Halts (mlet x <- p in q x) i
-    .
-
-    Lemma run_to_halts:
-      forall p i b,
-      Run p i (Halt b) ->
-      Halts p i.
-    Proof.
-      intros p i b Hr.
-      remember (Halt b).
-      generalize dependent b.
-      induction Hr; intros b' Hb; subst.
-      try (apply IHHr in Hdec; clear IHHr).
-      - constructor; eauto.
-      - constructor; eauto.
-      - constructor.
-      - econstructor; eauto.
-      - econstructor; eauto.
-      - inversion Hb.
-    Qed.
-
-    Lemma halts_to_run:
-      forall p i,
-      Halts p i ->
-      exists b, Run p i (Halt b).
-    Proof.
-      intros.
-      induction H;
-        try (destruct IHHalts as (b', IH));
-        try (exists b'; constructor; assumption; fail);
-        try (exists b; constructor; assumption; fail);
-        exists b'.
-      - eapply run_seq_cont; eauto.
-    Qed.
-
-    Lemma halts_rw:
-      forall p i,
-      (exists b, Run p i (Halt b)) <-> Halts p i.
-    Proof.
-      split; intros.
-      - destruct H. eauto using run_to_halts.
-      - auto using halts_to_run.
-    Qed.
-
-    Lemma decider_to_halts:
-      forall p,
-      Decider p ->
-      forall i,
-      Halts p i.
-    Proof.
-      intros.
-      rewrite <- halts_rw.
-      auto.
-    Qed.
-
-    Lemma halts_to_decider:
-      forall p,
-      (forall i, Halts p i) ->
-      Decider p.
-    Proof.
-      intros.
-      unfold Decider.
-      intros.
-      rewrite halts_rw.
-      auto.
-    Qed.
-
-    Lemma decides_to_halts:
-      forall p L,
-      Decides p L ->
-      forall i,
-      Halts p i.
-    Proof.
-      intros.
-      destruct H.
-      auto using decider_to_halts.
-    Qed.
- 
-  End HALTS.
 
   (** Tactics that simplify `Run` objects in the assumptions. *)
 
@@ -899,6 +1148,14 @@ Require Import Coq.Logic.Classical_Prop.
       | Run (Read _) _ _ => idtac
       | Run (Tur _) _ _ => idtac
       | Run (Ret _) _ _ => idtac
+      | Loop (Call _ _) _ => idtac
+      | Loop (Read _) _ => idtac
+      | Loop (Tur _) _ => idtac
+      | Loop (Ret _) _ => idtac
+      | Halt (Call _ _) _ => idtac
+      | Halt (Read _) _ => idtac
+      | Halt (Tur _) _ => idtac
+      | Halt (Ret _) _ => idtac
       | _ => fail
     end;
     inversion H; subst; clear H
@@ -914,14 +1171,6 @@ Require Import Coq.Logic.Classical_Prop.
         | false = true => idtac
         | true = false => idtac
 
-        | Halt true = Halt true => idtac
-        | Halt false = Halt false => idtac
-        | Loop = Loop => idtac
-
-        | Halt true = Halt false => idtac
-        | Halt false = Halt true => idtac
-        | Halt _ = Loop => idtac
-        | Loop = Halt _ => idtac
         | False => idtac
         | _ => fail
         end; inversion H
@@ -938,17 +1187,21 @@ Require Import Coq.Logic.Classical_Prop.
   Ltac run_simpl_norm :=
     match goal with
     | [ H: ?x = ?x |- _] => clear H
+    | [ H1: Negative ?p ?i, H2: Run ?p ?i true |- _ ] =>
+      rewrite negative_rw in H1; contradiction
+    | [ H1: Run ?p ?i _, H2: Loop ?p ?i |- _ ] =>
+      apply run_to_halt in H1;
+      rewrite loop_rw in H2; contradiction 
+    | [ H1: Halt ?p ?i, H2: Loop ?p ?i |- _ ] =>
+      rewrite loop_rw in H2; contradiction
     | [ H1: Run ?m ?i ?r1, H2: Run ?m ?i ?r2  |- _] =>
       assert (r1 = r2) by eauto using run_fun;
       subst; clear H1
-    | [ H: Halt _ = Halt _ |- _ ] => inversion H; subst; clear H
     | [ H1: Exec ?m ?i ?r1, H2: Exec ?m ?i ?r2  |- _] =>
       assert (r1 = r2) by eauto using exec_fun;
       subst; clear H1
     | [ H: true = _ |- _ ] => symmetry in H
     | [ H: false = _ |- _ ] => symmetry in H
-    | [ H: Halt _ = _ |- _ ] => symmetry in H
-    | [ H: Loop = _ |- _ ] => symmetry in H
     | [ H: negb _ = true |- _ ] => apply negb_true_iff in H; subst
     | [ H: negb _ = false |- _ ] => apply negb_false_iff in H; subst
     | [ H: andb _ _ = true |- _] => apply andb_prop in H
